styling fixes

Cslib/ConcurrencyTheory/CCS/Semantics.lean
@@ -23,26 +23,28 @@ open Process
 
 /-- The transition relation for CCS. This is a direct formalisation of the one found in
 [Sangiorgi2011]. -/
-inductive tr : Process Name Constant → Act Name → Process Name Constant → Prop where
-| pre : tr (pre μ p) μ p
-| parL : tr p μ p' → tr (par p q) μ (par p' q)
-| parR : tr q μ q' → tr (par p q) μ (par p q')
-| com : tr p μ p' → tr q μ.co q' → tr (par p q) Act.τ (par p' q')
-| choiceL : tr p μ p' → tr (choice p q) μ p'
-| choiceR : tr q μ q' → tr (choice p q) μ q'
-| res : μ ≠ Act.name a → μ ≠ Act.coname a → tr p μ p' → tr (res a p) μ (res a p')
-| const : defs k p → tr p μ p' → tr (const k) μ p'
+inductive Tr : Process Name Constant → Act Name → Process Name Constant → Prop where
+  | pre : Tr (pre μ p) μ p
+  | parL : Tr p μ p' → Tr (par p q) μ (par p' q)
+  | parR : Tr q μ q' → Tr (par p q) μ (par p q')
+  | com : Tr p μ p' → Tr q μ.co q' → Tr (par p q) Act.τ (par p' q')
+  | choiceL : Tr p μ p' → Tr (choice p q) μ p'
+  | choiceR : Tr q μ q' → Tr (choice p q) μ q'
+  | res : μ ≠ Act.name a → μ ≠ Act.coname a → Tr p μ p' → Tr (res a p) μ (res a p')
+  | const : defs k p → Tr p μ p' → Tr (const k) μ p'
 
 /-- The `LTS` of CCS. -/
-def lts : LTS (Process Name Constant) (Act Name) := {
-  tr := @CCS.tr Name Constant defs
-}
+def lts : LTS (Process Name Constant) (Act Name) where
+  Tr := @CCS.Tr Name Constant defs
+
+instance : HasTau (Act Name) where
+  τ := Act.τ
 
 /-- A process is (successfully) terminated if it is a composition of `nil`s. -/
 inductive Terminated : Process Name Constant → Prop where
-| nil : Terminated Process.nil
-| par : Terminated p → Terminated q → Terminated (par p q)
-| choice : Terminated p → Terminated q → Terminated (choice p q)
-| res : Terminated p → Terminated (res a p)
+  | nil : Terminated Process.nil
+  | par : Terminated p → Terminated q → Terminated (par p q)
+  | choice : Terminated p → Terminated q → Terminated (choice p q)
+  | res : Terminated p → Terminated (res a p)
 
 end CCS
